Commit for synching.

reflex/coq/ReflexCar.v
@@ -5,6 +5,7 @@ Require Import ReflexBase.
 Require Import ReflexDenoted.
 Require Import ReflexFin.
 Require Import ReflexFrontend.
+Require Import ReflexHVec.
 Require Import ReflexIO.
 Require Import ReflexVec.
 
@@ -12,23 +13,20 @@ Open Scope string_scope.
 
 Module SystemFeatures <: SystemFeaturesInterface.
 
-Definition NB_MSG : nat := 5.
+Definition NB_MSG : nat := 6.
 
 Definition PAYD : vvdesc NB_MSG := mk_vvdesc
-  [ ("CrashDetected", [])
-  ; ("Stop",          [])
-  ; ("Unlock",        [])
-  ; ("NewLocation",   [num_d; num_d])
-  ; ("Speed",  [num_d])
+  [
+    ("Crash",   []);
+    ("Acceleration",   []);
+    ("DoorsOpen",   []);
+    ("UnlockDoors",   []);
+    ("VolumeUp",   []);
+    ("VolumeDown",   [])
   ].
 
-Notation CrashDetected := 0%fin (only parsing).
-Notation Stop := 1%fin (only parsing).
-Notation Unlock := 2%fin (only parsing).
-Notation NewLocation := 3%fin (only parsing).
-Notation Speed := 4%fin (only parsing).
+Inductive COMPT' : Type := Engine | Doors | Radio.
 
-Inductive COMPT' : Type := Control | Body | Telematics | Media | KeylessEntry.
 Definition COMPT := COMPT'.
 
 Definition COMPTDEC : forall (x y : COMPT), decide (x = y).
@@ -36,23 +34,40 @@ Proof. decide equality. Defined.
 
 Definition COMPS (t : COMPT) : compd :=
   match t with
-  | Control => mk_compd "Control" "test/echo-00/test.py" [] (mk_vdesc [])
-  | Body => mk_compd "Body" "test/echo-00/test.py" [] (mk_vdesc [])
-  | Telematics => mk_compd "Telematics" "test/echo-00/test.py" [] (mk_vdesc [])
-  | Media => mk_compd "Media" "test/echo-00/test.py" [] (mk_vdesc [])
-  | KeylessEntry => mk_compd "KeylessEntry" "test/echo-00/test.py" [] (mk_vdesc [])
+  | Engine => mk_compd
+                "Engine" "engine.c" []
+                (mk_vdesc [])
+  | Doors => mk_compd
+                "Doors"  "doors.c"      []
+                (mk_vdesc [])
+  | Radio => mk_compd
+                "Radio"  "radio.c"    []
+                (mk_vdesc [])
   end.
 
-Definition KSTD : vcdesc COMPT := mk_vcdesc [(*crashed*)Desc _ num_d
-                                            ;(*locked*) Desc _ num_d].
+Notation Crash        := 0%fin (only parsing).
+Notation Acceleration       := 1%fin (only parsing).
+Notation DoorsOpen       := 2%fin (only parsing).
+Notation UnlockDoors       := 3%fin (only parsing).
+Notation VolumeUp       := 4%fin (only parsing).
+Notation VolumeDown      := 5%fin (only parsing).
 
 Definition IENVD : vcdesc COMPT := mk_vcdesc
-  [ Comp _ Control;
-    Comp _ Body;
-    Comp _ Telematics;
-    Comp _ Media;
-    Comp _ KeylessEntry
+  [ Comp _ Engine; Comp _ Doors; Comp _ Radio ].
+
+Notation v_env_engine := 0%fin (only parsing).
+Notation v_env_doors  := 1%fin (only parsing).
+Notation v_env_radio  := 2%fin (only parsing).
+
+Definition KSTD : vcdesc COMPT := mk_vcdesc
+  [ Comp _ Engine
+  ; Comp _ Doors
+  ; Comp _ Radio
   ].
+
+Notation v_st_engine        := 0%fin (only parsing).
+Notation v_st_doors         := 1%fin (only parsing).
+Notation v_st_radio         := 2%fin (only parsing).
 
 End SystemFeatures.
 
@@ -61,177 +76,60 @@ Import SystemFeatures.
 Module Language := MkLanguage(SystemFeatures).
 
 Import Language.
-(*
+
 Module Spec <: SpecInterface.
 
 Include SystemFeatures.
 
 Definition INIT : init_prog PAYD COMPT COMPS KSTD IENVD :=
-  seq (spawn IENVD _ Control tt None (Logic.eq_refl _))
-  (seq (spawn IENVD _ Body tt (Some None) (Logic.eq_refl _))
-  (seq (spawn IENVD _ Telematics tt (Some (Some None)) (Logic.eq_refl _))
-  (seq (spawn IENVD _ Media tt (Some (Some (Some None))) (Logic.eq_refl _))
-  (seq (spawn IENVD _ KeylessEntry tt (Some (Some (Some (Some None)))) (Logic.eq_refl _))
-  nop)))).
+   seq (spawn _ IENVD Engine tt v_env_engine (Logic.eq_refl _))
+  (seq (stupd _ IENVD v_st_engine (i_envvar IENVD v_env_engine))
+  (seq (spawn _ IENVD Doors  tt v_env_doors  (Logic.eq_refl _))
+  (seq (stupd _ IENVD v_st_doors (i_envvar IENVD v_env_doors))
+  (seq (spawn _ IENVD Radio  tt v_env_radio  (Logic.eq_refl _))
+       (stupd _ IENVD v_st_radio (i_envvar IENVD v_env_radio)))))).
 
-(*(*Something stupid*)
-Section Stupid.
-
-Variable NB_COMPT : nat.
-
-Definition desc := fin NB_COMPT.
-
-Print hdlr_prog.
-Print mk_vvdesc.
-Definition sdenote_desc (d : desc) :=
-Definition msg_handler (tag : fin NB_MSG) : Type := 
-
-End Stupid.
-(*End something stupid*)*)
-
+Open Scope hdlr.
 Definition HANDLERS : handlers PAYD COMPT COMPS KSTD :=
-  fun m cc =>
-  let (ct, _, _) := cc in
-  match m as _m return forall (EQ : _m = m), _ with
-  | {| tag := t; pay := p |} =>
+  fun t ct =>
   match ct as _ct, t as _t return
-    forall _p, Build_msg PAYD _t _p = m -> s[[ comp_conf_desc _ _ _ct ]] -> _
+    {prog_envd : vcdesc COMPT & hdlr_prog PAYD COMPT COMPS KSTD _ct _t prog_envd}
   with
-  | _, (Some (Some (Some (Some (Some bad))))) => fun _ _ _ => match bad with end
-  | _, _ => fun p EQ =>
-    let envd := existT _ 0 tt in
-    existT (fun d => hdlr_prog PAYD COMPT COMPS KSTD cc _ d) envd (
-      seq (send envd _ _ ccomp None (mvar EQ None, tt))
-      nop
-    )
-  end p
-  end (Logic.eq_refl m).
+     | Engine, Crash =>
+       [[ mk_vcdesc [] :
+          send (stvar v_st_doors) UnlockDoors tt
+       ]]
+     | Engine, Acceleration =>
+       [[ mk_vcdesc [] :
+          send (stvar v_st_radio) VolumeUp tt
+       ]]
+     | Doors, DoorsOpen =>
+       [[ mk_vcdesc [] :
+          send (stvar v_st_radio) VolumeDown tt
+       ]]
+     | _, _ => [[ mk_vcdesc [] : nop ]]
+    end.
 
-Require Import NonInterference.
+Require Import NIExists.
+Require Import PruneFacts.
 
-Require Import Ynot.
-
-Ltac destruct_fin f :=
-  match type of f with
-  | False => destruct f
-  | _ => let f' := fresh "f" in
-         destruct f as [ f' | ]; [destruct_fin f' | ]
+Definition clblr (c : comp COMPT COMPS) :=
+  match comp_type _ _ c with
+  | Engine => true
+  | _      => false
   end.
 
-Ltac destruct_pay pay :=
-  compute in pay;
-  match type of pay with
-  | unit => idtac
-  | _ => let a := fresh "a" in
-         let b := fresh "b" in
-         destruct pay as [a b]; simpl in a; destruct_pay b
-  end.
+Definition vlblr (f : fin (projT1 KSTD)) := false.
 
-Ltac destruct_msg :=
-  match goal with
-  | [ m : msg _ |- _ ]
-      => let tag := fresh "tag" in
-         let pay := fresh "pay" in
-         destruct m as [tag pay]; destruct_fin tag;
-         destruct_pay pay
-  end.
+Local Opaque str_of_string.
 
-(*Destructs num, str, or fd equalities in the context.*)
-Ltac destruct_eq H :=
-  repeat match type of H with
-         | context[if ?x then _ else _ ]
-           => destruct x
-         end.
- (* repeat match type of H with
-         | context[num_eq ?a ?b]
-           => destruct (num_eq a b); simpl in *
-         | context[str_eq ?a ?b]
-           => destruct (str_eq a b); simpl in *
-         | context[fd_eq ?a ?b]
-           => destruct (fd_eq a b); simpl in *
-         end.*)
+Theorem ni : NI PAYD COMPT COMPTDEC COMPS
+  IENVD KSTD INIT HANDLERS clblr vlblr.
+Proof.
+  ni.
+Qed.
 
-Ltac destruct_input input :=
-  simpl in input; (*compute in input;*)
-  match type of input with
-  | unit => idtac
-  | _ => let x := fresh "x" in
-         let input' := fresh "input'" in
-         destruct input as [x input']; destruct_input input'
-  end.
+End Spec.
 
-Ltac unpack_inhabited :=
-  repeat match goal with
-         | [ H : ktr _ _ _ _ _ = inhabits ?tr |- _ ]
-           => simpl in H; apply pack_injective in H; subst tr
-         end.
-
-Ltac destruct_comp :=
-  match goal with
-  | [ c : Reflex.comp _ _ |- _ ]
-      => destruct c
-  end.
-
-Ltac unpack :=
-  match goal with
-  (*Valid exchange.*)
-  | [ s : Reflex.kstate _ _ _ _, s' : Reflex.kstate _ _ _ _ |- _ ]
-    => match goal with
-       | [ _ : kstate_run_prog _ _ _ _ _ _ _ _ s _ = s' |- _ ]
-         => subst s; subst s'
-       end
-  (*Initialization.*)
-  | [ s : Reflex.init_state _ _ _ _ _ |- _ ]
-    => match goal with
-         | [ H : s = Reflex.init_state_run_cmd _ _ _ _ _ _ _ _ |- _ ]
-           => subst s
-       end
-  (*Bogus msg*)
-  end; unpack_inhabited.
-
-Ltac spawn_call :=
-      match goal with
-      | [ Hcall : call_ok _ _ _ _ _ _ |- call_ok _ _ _ _ _ _ ]
-          => repeat apply call_ok_sub in Hcall; try assumption;
-             apply call_ok_sym in Hcall; try assumption;
-             repeat apply call_ok_sub in Hcall; try assumption;
-             apply call_ok_sym; try assumption
-      | [ Hspawn : spawn_ok _ _ _ _ _ _ |- spawn_ok _ _ _ _ _ _ ]
-          => repeat apply spawn_ok_sub in Hspawn; try assumption;
-             apply spawn_ok_sym in Hspawn; try assumption;
-             repeat apply spawn_ok_sub in Hspawn; try assumption;
-             apply spawn_ok_sym; try assumption
-      end.
-
-Ltac high_steps :=
-  intros;
-  match goal with
-  | [ IH : NonInterferenceSt _ _ _ _ _ _ _ _ |- _ ]
-    => unfold NonInterferenceSt in *; intros;
-       match goal with
-       | [ Hve1 : ValidExchange _ _ _ _ _ _ _ _ _ _,
-           Hve2 : ValidExchange _ _ _ _ _ _ _ _ _ _,
-           Hins : inputs _ _ _ _ _ = inputs _ _ _ _ _,
-           Hhigh : _ _ = true |- _ ]
-         => inversion Hve1; inversion Hve2;
-            destruct_msg; destruct_comp; repeat unpack;
-             simpl in *; rewrite Hhigh in *; inversion Hins;
-            f_equal; auto; apply IH; auto; try spawn_call
-       end
-  end.
-
-Ltac low_step :=
-  intros;
-  match goal with
-  | [ IH : NonInterferenceSt _ _ _ _ _ _ _ _ |- _ ]
-    => unfold NonInterferenceSt in *; intros;
-       match goal with
-       | [ Hve : ValidExchange _ _ _ _ _ _ _ _ _ _,
-           Hlow : _ _ = false |- _ ]
-         => inversion Hve; destruct_msg; destruct_comp; repeat unpack;
-            simpl in *; rewrite Hlow in *; apply IH; auto; try spawn_call
-       end
-  end.
-
-Ltac ni :=
-  apply ni_suf; [high_steps | low_step].*)
+Module Main := MkMain(Spec).
+Import Main.
