reflex/coq/ReflexSSH.v
@@ -146,246 +146,287 @@ Import SystemFeatures.
 Module Language := MkLanguage(SystemFeatures).
 
 Import Language.
-(*
+
 Module Spec <: SpecInterface.
 
 Include SystemFeatures.
 
 Definition INIT : init_prog PAYD COMPT COMPS KSTD IENVD :=
-  [ fun s => spawn IENVD _ System (str_of_string "System", tt) v_env_system (Logic.eq_refl _)
-  ; fun s => spawn IENVD _ Slave  tt                           v_env_slave  (Logic.eq_refl _)
-  ].
+   seq (spawn _ IENVD System (str_of_string "System", tt) v_env_system (Logic.eq_refl _))
+  (seq (stupd _ IENVD v_st_system (i_envvar IENVD v_env_system))
+  (seq (spawn _ IENVD Slave  tt                           v_env_slave  (Logic.eq_refl _))
+       (stupd _ IENVD v_st_slave (i_envvar IENVD v_env_slave)))).
 
 Definition system_pat := (Some (str_of_string "System"), tt).
 
 Definition exists_comp := exists_comp COMPT COMPTDEC COMPS.
 
+Open Scope hdlr.
 Definition HANDLERS : handlers PAYD COMPT COMPS KSTD :=
-  (fun m cc =>
-     let (ct, cf, _) := cc in
-     match tag PAYD m as _tm return
-       @sdenote _ SDenoted_vdesc (lkup_tag PAYD _tm) -> _
-     with
+  fun t ct =>
+  match ct as _ct, t as _t return
+    {prog_envd : vcdesc COMPT & hdlr_prog PAYD COMPT COMPS KSTD _ct _t prog_envd}
+  with
+     | Slave, LoginReq =>
+       [[ mk_vcdesc [] :
+          send (stvar v_st_system) SLoginReq (mvar LoginReq 0%fin, tt)
+       ]]
+     | System, SLoginResT =>
+       [[ mk_vcdesc [] :
+           seq (stupd _ _ v_st_auth_user     (mvar SLoginResT 0%fin))
+          (seq (stupd _ _ v_st_authenticated (nlit (num_of_nat 1)))
+               (send (stvar v_st_slave) LoginResT tt))
+       ]]
+     | System, SLoginResF =>
+       [[ mk_vcdesc [] :
+          send (stvar v_st_slave) LoginResF tt
+       ]]
+     | Slave, PubkeyReq =>
+       [[ mk_vcdesc [] :
+          send (stvar v_st_system) SPubkeyReq tt
+       ]]
+     | System, SPubkeyRes =>
+       [[ mk_vcdesc [] :
+          send (stvar v_st_slave) PubkeyRes (mvar SPubkeyRes 0%fin, tt)
+       ]]
+     | Slave, KeysignReq =>
+       [[ mk_vcdesc [] :
+          send (stvar v_st_system) SKeysignReq (mvar KeysignReq 0%fin, tt)
+       ]]
+     | System, SKeysignRes =>
+       [[ mk_vcdesc [] :
+          send (stvar v_st_slave) KeysignRes (mvar SKeysignRes 0%fin, tt)
+       ]]
+     | Slave, CreatePtyerReq =>
+       [[ mk_vcdesc [] :
+          ite (eq (stvar v_st_authenticated) (nlit (num_of_nat 0)))
+              (
+                nop
+              )
+              (
+                send (stvar v_st_system) SCreatePtyerReq (stvar v_st_auth_user, tt)
+              )
+       ]]
+     | System, SCreatePtyerRes =>
+       [[ mk_vcdesc [] :
+          send (stvar v_st_slave) CreatePtyerRes
+            (mvar SCreatePtyerRes 0%fin, (mvar SCreatePtyerRes 1%fin, tt))
+       ]]
+     | _, _ => [[ mk_vcdesc [] : nop ]]
+    end.
 
-     | LoginReq => fun pl =>
-       let envd := mk_vcdesc [] in
-       existT (fun d => hdlr_prog PAYD COMPT COMPS KSTD cc _ d) envd (
-         let (loginstr, _) := pl in
-         (fun st0 =>
-            [ fun s => sendall envd _
-                               (mk_comp_pat
-                                  System
-                                  (Some (comp_fd st0##v_st_system%kst))
-                                  (None, tt)
-                               )
-                               SLoginReq (slit loginstr, tt)
-            ]
-         )
-       )
+Require Import PolLang.
+Require Import ActionMatch.
 
-     | SLoginResT => fun pl =>
-       let envd := mk_vcdesc [] in
-       existT (fun d => hdlr_prog PAYD COMPT COMPS KSTD cc _ d) envd (
-         let (user, _) := pl in
-         (fun st0 =>
-            match ct with
-            | System =>
-              [ fun s => stupd envd _ v_st_auth_user     (slit user)
-              ; fun s => stupd envd _ v_st_authenticated (nlit (num_of_nat 1))
-              ; fun s => sendall envd _
-                                 (mk_comp_pat
-                                    Slave
-                                    (Some (comp_fd st0##v_st_slave%kst))
-                                    tt
-                                 )
-                                 LoginResT tt
-              ]
-            | _ =>
-              []
-            end
-         )
-       )
+Local Opaque str_of_string.
 
-     | SLoginResF => fun pl =>
-       let envd := mk_vcdesc [] in
-       existT (fun d => hdlr_prog PAYD COMPT COMPS KSTD cc _ d) envd (
-         (fun st0 =>
-            [ fun s => sendall envd _
-                       (mk_comp_pat
-                          Slave
-                          (Some (comp_fd st0##v_st_slave%kst))
-                          tt
-                       )
-                       LoginResF tt
-            ]
-         )
-       )
+Definition System_pat : conc_pat COMPT COMPS :=
+  Build_conc_pat COMPT COMPS System (Some (str_of_string "System"), tt).
 
-     | PubkeyReq => fun pl =>
-       let envd := mk_vcdesc [] in
-       existT (fun d => hdlr_prog PAYD COMPT COMPS KSTD cc _ d) envd (
-         (fun st0 =>
-            [ fun s => sendall envd _
-                               (mk_comp_pat
-                                  System
-                                  (Some (comp_fd st0##v_st_system%kst))
-                                  (None, tt)
-                               )
-                               SPubkeyReq tt
-            ]
-         )
-       )
+Theorem enable : forall st tr u,
+  Reach PAYD COMPT COMPTDEC COMPS KSTD IENVD INIT HANDLERS st ->
+  ktr _ _ _ _ st = inhabits tr ->
+  Enables PAYD COMPT COMPS COMPTDEC
+          (KORecv PAYD COMPT COMPS (Some System_pat)
+                   (Some (Build_opt_msg PAYD
+                                         SLoginResT (Some u, tt))))
+          (KOSend PAYD COMPT COMPS None
+                   (Some (Build_opt_msg PAYD
+                                         SCreatePtyerReq (Some u, tt))))
+          tr.
+Proof.
+  crush.
+(*Ltac match_releases :=
+  match goal with
+  | [ |- Enables _ _ _ _ _ _ nil ]
+      => constructor
+  (* Induction hypothesis.*)
+  | [ H : Reflex.ktr _ _ _ _ ?s = inhabits ?tr,
+      IH : forall tr', Reflex.ktr _ _ _ _ ?s = inhabits tr' ->
+                       Enables _ _ _ _ ?past ?future tr'
+                       |- Enables _ _ _ _ ?past ?future ?tr ]
+      => auto
+  (*Branch on whether the head of the trace matches.*)
+  | [ |- Enables ?pdv ?compt ?comps ?comptdec _ ?future (?act::_) ]
+      => (*let s := match goal with
+                  | [ _ : ktr _ _ _ _ ?s = inhabits _ |- _ ]
+                      => s
+                  | [ s : init_state _ _ _ _ _ |- _ ]
+                      => s
+                  end in*)
+         let H := fresh "H" in
+         pose proof (decide_act pdv compt comps comptdec future act) as H;
+         destruct H;
+         [ first [ contradiction | destruct_action_matches; contradiction |
+           (apply E_future; [ match_releases | (*try exists_past*) ]) ]
+         | first [ contradiction | destruct_action_matches; contradiction |
+           (apply E_not_future; [ match_releases | assumption ]) ] ]
+         (*In some cases, one branch is impossible, so contradiction
+           solves the goal immediately.
+           In other cases, there are variables in the message payloads,
+           so both branches are possible.*)
+  end.
+reach_induction; try abstract match_releases.
 
-     | SPubkeyRes => fun pl =>
-       let envd := mk_vcdesc [] in
-       existT (fun d => hdlr_prog PAYD COMPT COMPS KSTD cc _ d) envd (
-         let (pubkey, _) := pl in
-         (fun st0 =>
-            [ fun s => sendall envd _
-                               (mk_comp_pat
-                                  System
-                                  (Some (comp_fd st0##v_st_system%kst))
-                                  (None, tt)
-                               )
-                               SPubkeyRes (slit pubkey, tt)
-            ]
-         )
-       )
+match_releases.
+destruct_action_matches.
+Ltac releaser_match :=
+  simpl;
+  repeat match goal with
+         | [ |- exists past : Reflex.KAction _ _ _, (?act = _ \/ ?disj_R ) /\ ?conj_R ]
+           => solve [exists act; split; [left; try subst; auto | compute; try subst; auto] ] ||
+              apply cut_exists
+         end.
+releaser_match.
+clear_useless_hyps.
+generalize dependent tr.
+induction H.
+  abstract (intros; inversion H; subst s0; subst s; simpl in *;
+  uninhabit; impossible).
 
-     | KeysignReq => fun pl =>
-       let envd := mk_vcdesc [] in
-       existT (fun d => hdlr_prog PAYD COMPT COMPS KSTD cc _ d) envd (
-         let (keystr, _) := pl in
-         (fun st0 =>
-            [ fun s => sendall envd _
-                               (mk_comp_pat
-                                  System
-                                  (Some (comp_fd st0##v_st_system%kst))
-                                  (None, tt)
-                               )
-                               SKeysignReq (slit keystr, tt)
-            ]
-         )
-       )
+  inversion H0. subst s'0. subst s'.
+  Ltac leaf_solve :=
+  simpl; try destruct_ite; simpl; intros;
+  try abstract (
+  uninhabit;
+  match goal with
+  | [ _ : Reflex.InitialState _ _ _ _ _ _ _ _ _ |- _ ]
+    => try subst; simpl in *;
+       try solve [ impossible
+                 | releaser_match ]
+  | [ _ : Reflex.ValidExchange _ _ _ _ _ _ _ _ _ _ _ |- _ ]
+    => try subst; simpl in *;
+       try solve [ impossible
+                 | use_IH_releases
+                 | releaser_match
+                 (*| exists_past*)]
+        (*destruct_eq might have created contradictions
+           with previous calls of destruct_eq*)
+  | [ _ : Reflex.BogusExchange _ _ _ _ _ _ _ _ |- _ ]
+    => try subst; simpl in *; use_IH_releases
+  | _ => idtac
+  end).
 
-     | SKeysignRes => fun pl =>
-       let envd := mk_vcdesc [] in
-       existT (fun d => hdlr_prog PAYD COMPT COMPS KSTD cc _ d) envd (
-         let (signedkey, _) := pl in
-         (fun st0 =>
-            [ fun s => sendall envd _
-                               (mk_comp_pat
-                                  System
-                                  (Some (comp_fd st0##v_st_system%kst))
-                                  (None, tt)
-                               )
-                               KeysignRes (slit signedkey, tt)
-            ]
-         )
-       )
+Ltac destruct_solve tag pay :=
+  match type of tag with
+  | False => contradiction
+  | _ => let tag' := fresh "tag" in
+          destruct tag as [tag' | ];
+          [ | try (destruct_pay pay; leaf_solve) ]
+          (*destruct_solve tag' pay*)
+  | _ => idtac
+  end.
+  destruct_comp; destruct m as [tag pay].
+  destruct_solve tag pay.
+  destruct_solve tag0 pay.
+  destruct_solve tag pay.
+  destruct_solve tag0 pay.
+Focus 2.
+simpl in *. unfold hdlrs in H1. destruct_comp. simpl in H1.
+uninhabit. try subst. idtac. use_IH_releases.
+  destruct_msg; destruct_comp.
+destruct s.
+destruct kst.
+destruct s1.
+destruct p.
+destruct p.
 
-     | CreatePtyerReq => fun pl =>
-       let envd := mk_vcdesc [] in
-       existT (fun d => hdlr_prog PAYD COMPT COMPS KSTD cc _ d) envd (
-         (fun st0 =>
-           if num_eq
-                (st0##v_st_authenticated%kst)
-                (num_of_nat 0)
-           then []
-           else [ fun s => sendall envd _
-                                   (mk_comp_pat
-                                      System
-                                      (Some (comp_fd st0##v_st_system%kst))
-                                      (None, tt)
-                                   )
-                                   SCreatePtyerReq (stvar v_st_auth_user, tt)
-                ]
-         )
-       )
+intros.
+  generalize dependent tr.
+ induction H.
+   unpack. abstract match_releases.
 
-     | SCreatePtyerRes => fun pl =>
-       let envd := mk_vcdesc [] in
-       existT (fun d => hdlr_prog PAYD COMPT COMPS KSTD cc _ d) envd (
-         match pl with
-         | (fd0, (fd1, _)) =>
-           (fun st0 =>
-              [ fun s => sendall envd _
-                                 (mk_comp_pat
-                                    System
-                                    (Some (comp_fd st0##v_st_system%kst))
-                                    (None, tt)
-                                 )
-                                 CreatePtyerRes (cfd, (cfd, tt))
-              ]
-           )
-         end
-       )
+   inversion H0. subst s'0. subst s'. 
 
-     (* not meant to be received by the kernel *)
-     | LoginResT => fun pl =>
-       let envd := mk_vcdesc [] in
-       existT (fun d => hdlr_prog PAYD COMPT COMPS KSTD cc _ d) envd (
-         (fun st0 => [])
-       )
+Ltac leaf_solve :=
+  simpl; try destruct_ite; simpl; intros; try abstract (uninhabit; match_releases).
 
-     | LoginResF => fun pl =>
-       let envd := mk_vcdesc [] in
-       existT (fun d => hdlr_prog PAYD COMPT COMPS KSTD cc _ d) envd (
-         (fun st0 => [])
-       )
+Ltac destruct_solve tag pay :=
+  match type of tag with
+  | False => contradiction
+  | _ => let tag' := fresh "tag" in
+          destruct tag as [tag' | ];
+          [ | try (destruct_pay pay; leaf_solve) ];
+          try (destruct_solve tag' pay)
+  end.
 
-     | PubkeyRes => fun pl =>
-       let envd := mk_vcdesc [] in
-       existT (fun d => hdlr_prog PAYD COMPT COMPS KSTD cc _ d) envd (
-         (fun st0 => [])
-       )
+destruct_comp; destruct m as [tag pay]. destruct_solve tag pay. destruct_solve tag pay.
 
-     | KeysignRes => fun pl =>
-       let envd := mk_vcdesc [] in
-       existT (fun d => hdlr_prog PAYD COMPT COMPS KSTD cc _ d) envd (
-         (fun st0 => [])
-       )
+Ltac releaser_match :=
+  simpl;
+  repeat match goal with
+         | [ |- exists past : Reflex.KAction _ _ _, (?act = _ \/ ?disj_R ) /\ ?conj_R ]
+           => solve [exists act; split; [left; try subst; auto | compute; try subst; auto] ] ||
+              apply cut_exists
+         end.
 
-     | CreatePtyerRes => fun pl =>
-       let envd := mk_vcdesc [] in
-       existT (fun d => hdlr_prog PAYD COMPT COMPS KSTD cc _ d) envd (
-         (fun st0 => [])
-       )
+Ltac exists_past :=
+  destruct_action_matches;
+  (*There may be conditions on s' (the intermediate state). We want
+    to use these conditions to derive conditions on s.*)
+  (*subst_states;*)
+  (*Try to match stuff at head of trace.*)
+  releaser_match;
+  (*This may not clear the old induction hypothesis. Does it matter?*)
+  clear_useless_hyps(*;
+  (*Should this take s as an argument?*)
+  reach_induction;
+  try abstract
+  (match goal with
+  | [ _ : Reflex.InitialState _ _ _ _ _ _ _ _ _ |- _ ]
+    => try subst; simpl in *;
+       try solve [ impossible
+                 | releaser_match ]
+  | [ _ : Reflex.ValidExchange _ _ _ _ _ _ _ _ _ _ _ |- _ ]
+    => try subst; simpl in *;
+       try solve [ impossible
+                 | use_IH_releases
+                 | releaser_match
+                 (*| exists_past*)]
+        (*destruct_eq might have created contradictions
+           with previous calls of destruct_eq*)
+  | [ _ : Reflex.BogusExchange _ _ _ _ _ _ _ _ |- _ ]
+    => try subst; simpl in *; use_IH_releases
+  | _ => idtac
+  end)*).
+simpl. intros; uninhabit.
+match_releases.
+idtac.
+destruct_action_matches.
+releaser_match.
+clear_useless_hyps.
+exists_past.
+generalize dependent tr.
+Ltac unpack :=
+  match goal with
+  | [ H : Reflex.InitialState _ _ _ _ _ _ _ _ ?s |- _ ]
+    => inversion H;
+       match goal with
+       | [ _ : ?s' = init_state_run_cmd _ _ _ _ _ _ _ _ _ |- _ ]
+         => subst s'; subst s
+       end
+  | [ H : Reflex.ValidExchange _ _ _ _ _ _ _ _ _ _ ?s |- _ ]
+    => destruct_msg; destruct_comp; inversion H;
+       match goal with
+       | [ _ : ?s' = mk_inter_ve_st _ _ _ _ _ _ _ _ |- _ ]
+         => subst s'; subst s
+       end
+  | [ H : Reflex.BogusExchange _ _ _ _ _ _ _ ?s |- _ ]
+    => inversion H; subst s
+  end; simpl; try destruct_ite_pol; simpl in *; intros; uninhabit.
+induction H; try unpack.
 
-     | SLoginReq => fun pl =>
-       let envd := mk_vcdesc [] in
-       existT (fun d => hdlr_prog PAYD COMPT COMPS KSTD cc _ d) envd (
-         (fun st0 => [])
-       )
+  impossible.
 
-     | SPubkeyReq => fun pl =>
-       let envd := mk_vcdesc [] in
-       existT (fun d => hdlr_prog PAYD COMPT COMPS KSTD cc _ d) envd (
-         (fun st0 => [])
-       )
-
-     | SKeysignReq => fun pl =>
-       let envd := mk_vcdesc [] in
-       existT (fun d => hdlr_prog PAYD COMPT COMPS KSTD cc _ d) envd (
-         (fun st0 => [])
-       )
-
-     | SCreatePtyerReq => fun pl =>
-       let envd := mk_vcdesc [] in
-       existT (fun d => hdlr_prog PAYD COMPT COMPS KSTD cc _ d) envd (
-         (fun st0 => [])
-       )
-
-     | (Some (Some (Some (Some (Some (Some (Some (Some (Some (Some (Some (Some (Some (Some (Some (Some (Some (Some bad)))))))))))))))))) => fun _ =>
-      match bad with end
-    end (pay PAYD m)
-  ).
+  destruct_msg; destruct_comp.
+    inversion H0. subst s'0. subst s'. simpl. try destruct_ite_pol. intros. uninhabit.*)
+Qed.
 
 End Spec.
 
 Module Main := MkMain(Spec).
 Import Main.
-
+(*
 Require Import PolLang.
 Require Import ActionMatch.
 Require Import Tactics.
